eager semantics was the right way to go

verif/Xor_verif.v
@@ -15,6 +15,7 @@ Require Import Values.
 Require Import Bitstream.
 
 Require Import EvalTac.
+Require Import Eager.
 
 Import HaskellListNotations.
 Open Scope string.
@@ -25,9 +26,9 @@ Require Import Xor.
 Definition decrypt : Expr := (ETApp (EVar (243,"decrypt")) (ETyp (TCon (TC (TCNum 3)) nil))).
 Definition encrypt : Expr := (ETApp (EVar (242,"encrypt")) (ETyp (TCon (TC (TCNum 3)) nil))).
 
-Notation "eval_expr* GE E V" := (eval_expr GE _ E V) (at level 99, only printing).
-Notation "vcons* V EXP" := (vcons V EXP _) (at level 98, only printing).
-Notation "force_list* V VS" := (force_list _ _ V VS) (at level 97, only printing).
+(* Notation "eval_expr* GE E V" := (eval_expr GE _ E V) (at level 99, only printing). *)
+(* Notation "vcons* V EXP" := (vcons V EXP _) (at level 98, only printing). *)
+(* Notation "force_list* V VS" := (force_list _ _ V VS) (at level 97, only printing). *)
 
 Lemma single_bit_roundtrip :
   forall (b b' : bool),
@@ -36,185 +37,261 @@ Proof.
   intros. destruct b; destruct b'; simpl; auto.
 Qed.
 
+Definition match_val {A B : Type} (a : A) (b : B) : Prop := True. (* TODO *)
+
+Lemma n_bits_destr :
+  forall n x,
+    n_bits (S n) x ->
+    exists b x',
+      x = (bit b) :: x' /\ n_bits n x'.
+Proof.
+  intros. inversion H. subst. eauto.
+Qed.
+
+(* we need an eager eqivalent for n_bits *)
+
+Ltac nb_destr :=
+  repeat (match goal with
+          | [ H : n_bits _ _ |- _ ] => eapply n_bits_destr in H
+          end);
+  repeat (match goal with
+         | [ H : exists _, _ |- _ ] => destruct H
+          end);
+  match goal with
+  | [ H : _ /\ _ |- _ ] => destruct H
+  end;
+  try match goal with
+      | [ H : n_bits O _ |- _ ] => inversion H; clear H
+      end.
+         
+Definition sempty : ident -> option strictval := fun x => None.
+
+
+
+Lemma n_bits_eval :
+  forall n x,
+    n_bits n x ->
+    exists v,
+      eager_eval_expr ge sempty (EList (map EValue x)) v.
+Proof.
+  induction 1; intros.
+  eexists. econstructor; eauto. simpl. econstructor.
+  destruct IHn_bits.
+  inversion H0.
+  eexists. simpl. econstructor. simpl. econstructor. econstructor. econstructor.
+  eauto. reflexivity.
+Qed.
+
+
+Lemma xor_bits_roundtrip :
+  forall n x y,
+    n <> O ->
+    n_bits n x ->
+    n_bits n y ->
+    forall vx vy,
+      eager_eval_expr ge sempty (EList (map EValue x)) vx ->
+      eager_eval_expr ge sempty (EList (map EValue y)) vy ->
+      exists halfway,
+        xor_sem vx vy = Some halfway /\ xor_sem halfway vy = Some vx.
+Proof.
+  induction n; intros. congruence.
+  destruct n.
+  clear IHn. 
+  - (* base case *)
+    inversion H0. subst. inversion H5. subst.
+    inversion H1. subst. inversion H6. subst.
+    clear H5 H6.
+    inversion H2. inversion H3. subst. inversion H5. inversion H10.
+    subst. inversion H9. inversion H15. subst. inversion H7. inversion H13.
+    subst. inversion H8. inversion H16. subst. unfold strict_list.
+    simpl. eexists; split. reflexivity.
+    simpl. rewrite single_bit_roundtrip. reflexivity.
+  - inversion H0. subst. clear H0.
+    inversion H1. subst. clear H1.
+    simpl in H2. simpl in H3.
+    inversion H2. inversion H3. subst.
+    inversion H1. inversion H10. subst.
+    
+    edestruct IHn. congruence. eapply H5. eapply H4. 
+    econstructor. eassumption. reflexivity.
+    econstructor. eassumption. reflexivity.
+    destruct H0.
+    simpl. rewrite H0.
+    inversion H7. inversion H13. subst.
+    inversion H12. inversion H18. subst. simpl.
+    eexists; split; try reflexivity.
+    simpl. rewrite H6.
+    rewrite single_bit_roundtrip. reflexivity.
+Qed.
+    
+
+Lemma xor_roundtrip_eager :
+  forall pt,
+    Forall (n_bits 8%nat) pt ->
+    forall k,
+      n_bits (8%nat) k ->
+      exists pt',
+        eager_eval_expr ge sempty (EApp (EApp decrypt (EList (map EValue k))) (EApp (EApp encrypt (EList (map EValue k))) (EList (map EList (map (map EValue) pt))))) pt' /\ match_val pt pt'.
+Proof.
+  induction 1; intros.
+  - repeat nb_destr; subst.
+    eexists; split.
+    unfold decrypt.
+    econstructor. econstructor. 
+    econstructor. eapply eager_eval_global_var.
+    simpl; eauto. unfold ge; unfold extend; simpl. reflexivity.
+    econstructor.
+    repeat econstructor; eauto.
+    econstructor.
+    econstructor. simpl.
+    repeat econstructor. reflexivity.
+    econstructor. e. e. unfold encrypt.
+    e. eapply eager_eval_global_var. reflexivity. reflexivity.
+    e. repeat e. e. repeat e.
+    e. e. e.
+    
+    e. repeat e. simpl. repeat e.
+    e. repeat e. simpl. repeat e.
+    (* TODO *)
+    simpl. unfold match_val. auto.
+
+  - remember H1 as Hkey; clear HeqHkey.
+    eapply IHForall in H1.
+    clear IHForall. destruct H1. destruct H1.
+    inversion H1. subst. clear H1.
+    unfold decrypt in *. unfold encrypt in *.
+    inversion H7. subst. clear H7.
+    inversion H4. subst. clear H4.
+    inversion H6. subst. clear H6.
+    inversion H4. subst. clear H4.
+    unfold sempty in *. congruence.
+    subst. clear H4.
+    clear H3.
+    unfold ge in H6; unfold extend in H6; simpl in H6; inversion H6; subst; clear H6.
+    inversion H12. subst. clear H12.
+    inversion H6. subst. clear H6.
+    inversion H14. subst. clear H14.
+    inversion H15. subst. clear H15.
+    inversion H13. subst. clear H13.
+    inversion H11. subst. clear H11.
+    inversion H4; try congruence. subst. clear H4.
+    inversion H6; try congruence. subst. clear H6.
+    inversion H11. subst. clear H11.
+    Focus 2. subst. unfold extend in H3. simpl in H3. congruence.
+    unfold extend in H4. simpl in H4. inversion H4. subst. clear H4.
+    inversion H8. subst. clear H8.
+    
+    inversion H5. subst. clear H5.
+    inversion H6. subst. clear H6.
+    inversion H5. subst. clear H5.
+    unfold sempty in H6. simpl in H6. congruence.
+    subst. clear H5. clear H4.
+    unfold ge in H6. unfold extend in H6. simpl in H6. inversion H6; subst; clear H6.
+    inversion H15. subst. clear H15.
+    inversion H16. subst. clear H16.
+    inversion H12. subst. clear H12.
+    inversion H6. subst. clear H6.
+    inversion H14. subst. clear H14.
+    rewrite list_of_strictval_of_strictlist in H13. inversion H13. subst. clear H13.
+    inversion H9. subst. clear H9.
+    inversion H5; try congruence. subst. clear H5.
+    inversion H6; try congruence. subst. clear H6.
+    inversion H9. subst. clear H9.
+    Focus 2. subst. unfold extend in H4. simpl in H4. congruence.
+    unfold extend in H5. simpl in H5. inversion H5. clear H5. subst.
+    rewrite list_of_strictval_of_strictlist in H13. inversion H13. subst. clear H13.
+    assert (av = av1). {
+      repeat nb_destr; subst.
+      inversion H11. subst. clear H11.
+      inversion H10. subst. clear H10.
+      clear -H1 H4.
+      repeat (match goal with
+              | [ H : Forall2 _ _ _ |- _ ] => inversion H; subst; clear H
+              end).
+      repeat match goal with
+             | [ H : eager_eval_expr _ _ (EValue _) _ |- _ ] => inversion H; subst; clear H
+             end.
+      repeat match goal with
+             | [ H : strict_eval_val _ (vcons _ _ _) _ |- _ ] => inversion H; subst; clear H
+             | [ H : strict_eval_val _ (bit _) _ |- _ ] => inversion H; subst; clear H
+             | [ H : strict_eval_val _ vnil _ |- _ ] => inversion H; subst; clear H
+             end.
+      reflexivity.
+
+    } idtac.
+    subst. clear H11.
+    
+    (* need this *)
+    assert (exists x', eager_eval_expr ge sempty (EList (map EValue x)) x'). {
+      eapply n_bits_eval; eauto.
+    } idtac.
+    destruct H1.
+    
+    
+
+    
+    assert (exists halfway, xor_sem x0 av1 = Some halfway /\ xor_sem halfway av1 = Some x0). {
+      eapply xor_bits_roundtrip. Focus 4. eassumption. Focus 4. eassumption.
+      Focus 2. eassumption.
+      Focus 2. eassumption.
+      congruence.
+    } idtac.
+    destruct H4. destruct H4.
+    
+    eexists; split.
+
+    e. e. e. eapply eager_eval_global_var. reflexivity. reflexivity.
+    e. repeat e.
+    e. eassumption.
+    e. simpl. e. e. e.
+    eapply eager_eval_global_var. reflexivity. reflexivity.
+    e. repeat e.
+    e. eassumption. e. e. econstructor.
+    eassumption.
+    eassumption. (* apply (part of) inductive hypothesis *)
+    
+    e. e. e. e. simpl. rewrite list_of_strictval_of_strictlist. reflexivity.
+    simpl. econstructor.
+    * econstructor.
+      econstructor. econstructor. eapply (eager_eval_global_var); try reflexivity.
+      unfold mb. simpl. econstructor. econstructor. econstructor. reflexivity.
+      econstructor. econstructor. econstructor. econstructor. reflexivity.
+      econstructor. econstructor. reflexivity.
+      econstructor. repeat econstructor. simpl. eassumption.
+    * eapply eager_eval_other_envs. eassumption.
+      clear -lv.
+      {
+        admit. (* tis true *)
+      }
+    * e. e. e. e. rewrite list_of_strictval_of_strictlist. reflexivity.
+      simpl. econstructor.
+      econstructor. econstructor. econstructor.
+      eapply (eager_eval_global_var); try reflexivity.
+      unfold mb. simpl. econstructor. econstructor. econstructor. reflexivity.
+      econstructor. econstructor. econstructor. econstructor. reflexivity.
+      econstructor. econstructor. reflexivity.
+      econstructor. repeat econstructor. simpl.
+      eassumption.
+      eapply eager_eval_other_envs. eassumption.
+      {
+        admit. (* this is true, prove later *)
+      }
+    * unfold match_val. auto. (* TODO *)
+
+Admitted.
+    
+
 
 Lemma xor_roundtrip :
   forall pt,
     Forall (n_bits 8%nat) pt ->
     forall k,
       n_bits (8%nat) k ->
-      exists ciphertext,
-        eval_expr ge empty (EApp (EApp encrypt (EValue (thunk_list k))) (EList (map EList (map (map EValue) pt))) ) ciphertext /\
-        exists v',
-          eval_expr ge empty (EApp (EApp decrypt (EValue (thunk_list k))) (EValue ciphertext)) v' /\
-          exists vls,
-            force_list ge empty v' vls /\
-            Forall2 (force_list ge empty) vls pt.
+      exists pt',
+        strict_eval_expr ge empty (EApp (EApp decrypt (EList (map EValue k))) (EApp (EApp encrypt (EList (map EValue k))) (EList (map EList (map (map EValue) pt))))) pt' /\ match_val pt pt'.
 Proof.
-  induction 1; intros;
-    do 9 match goal with
-         | [ H : n_bits _ _ |- _ ] => inversion H
-         end; subst.
-  - clear -H.
-    eexists. split.
-    e. e. e. g.
-    repeat e. 
-    repeat e. repeat e. repeat e.
-    repeat e. repeat e.
-    e. 
-    eapply eval_comp_imp_nil.
-    repeat e. simpl. omega.
-    eexists.  split.
-    e. e. e. g. e. e. e.
-    e. e. e. e. eapply eval_comp. eapply eval_comp_imp_nil.
-    repeat e. simpl. omega.
-
-    eexists. split.
-    e. e.
-    
-  - clear -H1 H H0 IHForall.
-    inversion H. inversion H3. inversion H6. inversion H9. inversion H12.
-    inversion H15. inversion H18. inversion H21. inversion H24. subst.
-    clear -H1 H H0 IHForall.
-    eapply IHForall in H1; eauto.
-    clear IHForall. destruct H1. destruct H1.
-    inversion H1. subst.
-    destruct H2. destruct H2. destruct H3. destruct H3.
-    inversion H7. subst.
-
-    init_globals ge.
-
-    eexists; split.
-    + e. (* run encrypt *)
-      -- e. simpl. e. g.
-         repeat e. repeat e. repeat e. repeat e.
-         repeat e.
-      -- simpl. e. e. e. repeat e. eassumption. (* use part of inductive hypothesis *)
-      -- e. e. e. eapply idx_last. e. e. e. e. e. e. e. e. e. repeat e.
-         e. e. e. e. e.
-         eapply eval_lift_binary_builtin.
-         simpl; auto. simpl. instantiate (3 := (EVar (3,"")) :: nil). reflexivity.
-         e. e. e. eapply eval_binary_over_bit_to_bit. simpl. reflexivity.
-         e. e.
-    +
-Admitted.
-(*      (* BELOW MIGHT BE RIGHT IDK *)
-      eexists; split. (* run decrypt *)
-      e. e. e. g.
-      e. repeat e. e. e. e. e. e. e.
-      e. eapply idx_last. e. e. e. e. e. e. e.
-      e. e. e. repeat e. repeat e.
-      e. e. e. e. e.
-      eapply eval_lift_binary_builtin.
-      simpl. auto.
-      simpl.
-      instantiate (3 := (EVar (3,"")) :: nil). reflexivity.
-      simpl. e. e. e. simpl.
-      eapply eval_binary_over_bit_to_bit. reflexivity. e. e.
-
-      * destruct vs.
-        -- (* encrypt/decrypt exactly one byte, nothing more *)
-          eexists. split.
-          e. eapply eval_comp_imp_nil. e. e. e. e.
-          eapply eval_comp_imp_nil. repeat e. simpl. omega.
-          e. simpl. omega.
-          e. simpl. e.
-          rewrite single_bit_roundtrip. e.
-          e. e. e. e. simpl. eapply eval_binary_over_bit_to_bit. reflexivity.
-          e. e. e. eapply eval_binary_over_bit_to_bit. reflexivity.
-          e. e. simpl.
-          rewrite single_bit_roundtrip. e.
-          e. e. e. e. eapply eval_binary_over_bit_to_bit. reflexivity.
-          e. e. e. eapply eval_binary_over_bit_to_bit. reflexivity.
-          simpl. e. e. simpl.
-          rewrite single_bit_roundtrip. e.
-          e. e. e. e. eapply eval_binary_over_bit_to_bit. reflexivity.
-          e. e. e. eapply eval_binary_over_bit_to_bit. reflexivity.
-          simpl. e. e. simpl.
-          rewrite single_bit_roundtrip. e.
-          e. e. e. e. eapply eval_binary_over_bit_to_bit. reflexivity.
-          e. e. e. eapply eval_binary_over_bit_to_bit. reflexivity.
-          simpl. e. e. simpl.
-          rewrite single_bit_roundtrip. e.
-          e. e. e. e. eapply eval_binary_over_bit_to_bit. reflexivity.
-          e. e. e. eapply eval_binary_over_bit_to_bit. reflexivity.
-          simpl. e. e. simpl.
-          rewrite single_bit_roundtrip. e.
-          e. e. e. e. eapply eval_binary_over_bit_to_bit. reflexivity.
-          e. e. e. eapply eval_binary_over_bit_to_bit. reflexivity.
-          simpl. e. e. simpl.
-          rewrite single_bit_roundtrip. e.
-          e. e. e. e. eapply eval_binary_over_bit_to_bit. reflexivity.
-          e. e. e. eapply eval_binary_over_bit_to_bit. reflexivity.
-          simpl. e. e. simpl.
-          rewrite single_bit_roundtrip. eapply force_cons.
-          eapply eval_lift_binary_nil. eapply eval_lift_binary_nil. e. e. e. e.
-          destruct l; simpl in H8; inversion H8. e.
-        -- (* inductive case, encrypt/decrypt one byte then apply IH *)
-          
-          simpl.
-          
-          destruct l; try solve [simpl in H8; inversion H8].
-          inversion H0. subst. inversion H11. inversion H10.
-          inversion H15. inversion H18. inversion H21.
-          inversion H24. inversion H27. inversion H30. inversion H33. subst.
-          clear H33 H27 H21 H15 H10 H18 H24 H30.
-          simpl in H8. simpl in H7. inversion H8. inversion H7.
-          subst.
-
-          inversion H14. subst.
-          destruct vs0; simpl in H20; try congruence.
-          inversion H20. subst.
-          inversion H10. subst.
-          inversion H21. subst.
-          inversion H23. subst.
-          inversion H25. subst.
-          inversion H27. subst.
-          inversion H29. subst.
-          inversion H31. subst.
-          inversion H33. subst.
-          inversion H35. subst.
-          clear H35.
-          inversion H32. subst.
-          inversion H30. subst.
-          inversion H28. subst.
-          inversion H26. subst.
-          inversion H24. subst.
-          inversion H22. subst.
-          inversion H19. subst.
-          inversion H17. subst.
-          
-          eexists. split.
-
-          eapply force_cons.
-
-          --- 
-            e. e. eapply idx_last. e. e.
-            e. e. e. e. e. e. 
-            e. e.
-            e. e. e. e.
-            e. e. e. repeat e. repeat e. e. e. e. e.
-            eapply eval_lift_binary_builtin. simpl. auto.
-            simpl. instantiate (3 := (EVar (3,""))::nil). reflexivity.
-            e. e. e.
-            eapply eval_binary_over_bit_to_bit.
-            simpl. reflexivity.
-            e. e. e. e. e. e. e. e. e. repeat e.
-            e. e. e. e. e.
-            eapply eval_lift_binary_builtin. simpl. auto.
-            simpl. instantiate (3 := (EVar (3,""))::nil). reflexivity.
-            e. e. e.
-            eapply eval_binary_over_bit_to_bit.
-            simpl. reflexivity.
-            e. e.
-
-          --- (* inductive hypothesis needs to be used here I think *)
-            
-            e. e. e. e. e. e. e. e. e. e. e. e.
-            e. e. e. e. e. e. e. e. e. e. e. e. e. e. e. e.
-            e. eapply eval_lift_binary_builtin.
-            e. simpl. instantiate (3 := (EVar (3,""))::nil). reflexivity.
-            e. e. e. eapply eval_binary_over_bit_to_bit. reflexivity.
-            e. e. e.
-            (* HERE *)
-            (* What are the useful hypotheses? *)
-            *)
+  intros. eapply xor_roundtrip_eager in H0; eauto.
+  destruct H0. destruct H0.
+  eapply eager_to_strict_lazy in H0; eauto.
+  unfold match_env. intros. unfold empty. unfold sempty. econstructor.
+Qed.
